merge trace & trace.valid

StackLean/Basic.lean
@@ -19,7 +19,7 @@ def LSet (α : Type) := { l : List α // List.Nodup l }
 instance : EmptyCollection (LSet α) where
   emptyCollection := ⟨[], by simp⟩
 
-instance [DecidableEq α] : Membership α (LSet α) where
+instance : Membership α (LSet α) where
   mem (t : LSet α) (v : α) := v ∈ t.val
 
 instance (t : LSet α) (v : α) [DecidableEq α] : Decidable (v ∈ t) :=
@@ -101,57 +101,66 @@ def Target.vars (target : Target) : LSet Var := target.args.vars ∪ target.live
 
 --- Traces ---
 
-inductive Trace where
-  | Lit : (stk : Stack) → Trace
-  | Swap : ℕ → Trace → Trace
-  | Dup : ℕ → Trace → Trace
-  | Pop : Trace → Trace
-  | Push : Word → Trace → Trace
-  | MarkJunk : ℕ → Trace → Trace
-  deriving Repr
+--inductive Trace where
+  --| Lit : (stk : Stack) → Trace
+  --| Swap : ℕ → Trace → Trace
+  --| Dup : ℕ → Trace → Trace
+  --| Pop : Trace → Trace
+  --| Push : Word → Trace → Trace
+  --| MarkJunk : ℕ → Trace → Trace
+  --deriving Repr
 
-def Trace.start : Trace → Stack
-  | .Lit s => s
-  | .Swap _ t => t.start
-  | .Dup _ t => t.start
-  | .Pop t => t.start
-  | .Push _ t => t.start
-  | .MarkJunk _ t => t.start
+--def Trace.start : Trace → Stack
+  --| .Lit s => s
+  --| .Swap _ t => t.start
+  --| .Dup _ t => t.start
+  --| .Pop t => t.start
+  --| .Push _ t => t.start
+  --| .MarkJunk _ t => t.start
 
 def List.swap {α : Type u} (xs : List α) (i j : ℕ) (hi : i < xs.length := by get_elem_tactic) (hj : j < xs.length := by get_elem_tactic) := (xs.set i xs[j]).set j xs[i]
 
-inductive Trace.valid : Trace → Stack → Prop where
-  | Lit : Trace.valid (.Lit s) s
+inductive Trace : Stack → Stack → Prop where
+  | Refl
+    : (s : Stack)
+    → Trace s s
   | Swap
-    : Trace.valid s res
-    → (hlen : res.length > idx)
-    → (hlo : 0 < idx)
-    → (hhi : idx < 17)
-    → Trace.valid (.Swap idx s) (res.swap 0 idx)
+    : (idx : ℕ)
+    → (hlen : idx < prev.length)
+    → (hidx : 1 ≤ idx ∧ idx < 17)
+    → Trace s prev
+    → Trace s (prev.swap 0 idx)
   | Dup
-    : Trace.valid s res
-    → (hlen : idx < res.length)
-    → (hlo : 1 ≤ idx)
-    → (hhi : idx < 17)
-    → Trace.valid (.Dup idx s) (res[idx] :: res)
+    : (idx : ℕ)
+    → (hlen : idx < prev.length)
+    → (hidx : 1 ≤ idx ∧ idx < 17)
+    → Trace s prev
+    → Trace s (prev[idx] :: prev)
   | Pop
-    : Trace.valid s res
-    → (hlen : 0 < res.length)
-    → Trace.valid (.Pop s) res.tail
+    : (hlen : 0 < prev.length)
+    → Trace s prev
+    → Trace s prev.tail
   | Push
-    : Trace.valid s res
-    → Trace.valid (.Push word s) (.Lit word :: res)
+    : (w : Word)
+    → Trace s prev
+    → Trace s (.Lit w :: prev)
   | MarkJunk
-    : Trace.valid s res
-    → (hlen : idx < res.length)
-    → Trace.valid (.MarkJunk idx s) (res.set idx .Junk)
+    : (idx : ℕ)
+    → (hlen : idx < prev.length)
+    → Trace s prev
+    → Trace s (prev.set idx .Junk)
 
 
 -- apply theorems --
 
 -- dup grows stack size by 1
-theorem apply_dup_grows_stack (stack : Stack) (idx : ℕ) (heval : Trace.valid (.Dup idx (.Lit stack)) res) : res.length = stack.length + 1 := match heval with
-  | .Dup .Lit hlen hlo hhi => by simp_all
+--theorem apply_dup_grows_stack (start : Stack) (finish : Stack) (idx : ℕ) (hlen : idx < start.length) (hidx : 1 ≤ idx ∧ idx < 17) : Trace.Dup idx hlen hidx (.Refl start) : Trace start finish := by sorry
+
+/-
+
+theorem apply_dup_grows_stack (start : Stack) (finish : Stack) (idx : ℕ) (hlen : idx < start.length) (hidx : 1 ≤ idx ∧ idx < 17) (trace : Trace start finish) :
+    trace = .Dup idx hlen hidx (.Refl start) → finish.length = start.length + 1 := by
+      sorry
 
 
 -- applying swap at the same idx twice is a noop
@@ -164,6 +173,7 @@ theorem apply_swap_inv (stack : Stack) (idx : ℕ) (heval : Trace.valid (.Lit st
       simp_all [List.getElem?_set]
       split_ifs <;> simp_all
       exact List.getElem_eq_iff ?_
+-/
 
 --- Stack Shuffling ---
 
@@ -218,23 +228,23 @@ abbrev input_contains_all_target_vars (input : Stack) (target : Target) : Prop :
 instance (input : Stack) (target : Target) : Decidable (input_contains_all_target_vars input target) :=
   inferInstanceAs (Decidable (target.vars ⊆ input.vars))
 
-inductive ShuffleResult where
+inductive ShuffleResult (start : Stack) where
   | StackTooDeep
   | ForbiddenState
-  | ResultStack (trace : Trace) (finish : Stack) (valid : Trace.valid trace finish)
+  | ResultStack (finish : Stack) (trace : Trace start finish)
   deriving Repr
 
 mutual
 
 -- TODO: target can only be reached from stack if the variable set of target ⊆ the variable set of stack
-def shuffle (stack : Stack) (target : Target) (precondition : input_contains_all_target_vars stack target) : ShuffleResult
-  := shuffle.go (.Lit stack) .Lit target
+def shuffle (stack : Stack) (target : Target) (precondition : input_contains_all_target_vars stack target) : ShuffleResult stack
+  := shuffle.go stack stack (.Refl stack) target
 
 @[simp]
-def shuffle.go  (trace : Trace) (valid : Trace.valid trace state) (target : Target) : ShuffleResult :=
+def shuffle.go (start : Stack) (state : Stack) (trace : Trace start state) (target : Target) : ShuffleResult start :=
   if args_is_correct state target then
     if tail_is_compatible state target
-    then .ResultStack trace _ valid
+    then .ResultStack state trace
     else .StackTooDeep
 
   -- if we have too much stuff
@@ -242,7 +252,7 @@ def shuffle.go  (trace : Trace) (valid : Trace.valid trace state) (target : Targ
     if hcan_pop : input_contains_all_target_vars state.tail target then
       have : distance (List.tail state) target < distance state target := by
         clear hcan_pop; simp [distance]; split_ifs <;> grind
-      shuffle.go (.Pop trace) (.Pop valid (by omega)) target
+      shuffle.go start state.tail (.Pop (by omega) trace) target
     else
       .StackTooDeep
 
@@ -265,21 +275,37 @@ theorem shuffle_correct (stack : Stack) (target : Target) (hvars : input_contain
    -- the result of a shuffle is either:
    match shuffle stack target hvars with
      -- a valid sequence of ops from the input to a result stack compatible with the target
-     | .ResultStack trace finish valid => trace.start = stack ∧ is_compatible finish target
+     | .ResultStack finish trace => is_compatible finish target
      -- a stack too deep
      | .StackTooDeep => True
      -- we never enter the forbidden state
      | .ForbiddenState => False
    := by
-      unfold shuffle
       induction stack with
-      | nil => simp [shuffle.go]; split_ifs <;> simp_all [Trace.start]
+      | nil => simp [shuffle, shuffle.go]; split_ifs <;> simp_all
       | cons hd tl ih =>
+        unfold shuffle
         unfold shuffle.go
         split_ifs with hargs htail hsz hcan_pop
-        · simp [Trace.start]; grind
+        · simp; grind
         · simp
-        ·
+        · change input_contains_all_target_vars tl target at hcan_pop
+          obtain ih' := ih hcan_pop
+          simp only [List.tail]
+          unfold shuffle at ih'
+
+          unfold shuffle.go
+
+          split_ifs
+          · simp; grind
+          · simp
+          ·
+            sorry
+          · simp
+
+
+
+
           sorry
         · simp
         · simp
